

\section{Proof of Proposition 2 and 3}

\begin{proof}[of Proposition 2]
	First, we list the inequalities: \begin{align*}
		& \begin{aligned}
			y_j + x'_j &\leq a\beta_j        &
			y_j &+ x'_j \geq (1-a)\alpha_j \\
			x'_j       &\leq a'\beta_j       & 
			x'_j       &\geq (1-a')\alpha_j \\
			\hat{y}_j  &\leq a\gamma_j       &
			\hat{y}_j  &\geq -a'\gamma_j \\
			\hat{y}_j  &\leq y_j + x'_j - (1-a)\alpha_j &
			\hat{y}_j  &\geq y_j + x'_j - a'\beta_j \\
			\hat{y}_j  &\leq -x'_j + a\beta_j &
			\hat{y}_j  &\geq -x'_j + (1-a')\alpha_j \\
			\hat{y}_j  &\leq y_j + (1-a)\gamma_j  &
			\hat{y}_j  &\geq y_j - (1-a')\gamma_j
		\end{aligned}
	\end{align*} 
	
	Follow the discuss in the proof of main text, we need to check the other inequalities of each cases.
	
 \textbf{$\mathbf{a = 0, a' = 0}$:}  In this case, the inequalities become: \begin{align*}
 	& \begin{aligned}
 		y_j + x'_j &\leq 0       &
 		y_j &+ x'_j \geq \alpha_j \\
 		x'_j       &\leq 0       & 
 		x'_j       &\geq \alpha_j \\
 		\hat{y}_j  &\leq 0       &
 		\hat{y}_j  &\geq 0 \\
 		\hat{y}_j  &\leq y_j + x'_j -\alpha_j &
 		\hat{y}_j  &\geq y_j + x'_j  \\
 		\hat{y}_j  &\leq -x'_j  &
 		\hat{y}_j  &\geq -x'_j + \alpha_j \\
 		\hat{y}_j  &\leq y_j + \gamma_j  &
 		\hat{y}_j  &\geq y_j - \gamma_j
 	\end{aligned}
 \end{align*} Now we can see, $y_j+x'_j\leq 0$ and $x'_j \leq 0$ (lines 1\&2), $\hat{y}_j=0$ (line 3). 
 
 For other 3 lines, by above discussing and the assumption of the proposition that $y_j \in [-\gamma_j, \gamma_j]$ and $x'_j,y_j+x'_j \in [\alpha_j,\beta_j]$, they are implied by the following inequalities respectively (one for one) \begin{align*}
 & \begin{aligned}
 	\hat{y}_j  \leq 0 &\leq y_j + x'_j -\alpha_j &
 	\hat{y}_j  \geq 0 &\geq y_j + x'_j  \\
 	\hat{y}_j  \leq 0 &\leq -x'_j  &
 	\hat{y}_j  \geq 0 &\geq -x'_j + \alpha_j \\
 	\hat{y}_j  \leq 0 &\leq y_j + \gamma_j  &
 	\hat{y}_j  \geq 0 &\geq y_j - \gamma_j
 \end{aligned}
 \end{align*} Therefore all 3 rest lines are tautology.
 
 
\textbf{$\mathbf{a = 1, a' = 0}$:} In this case, the inequalities become: \begin{align*}
	& \begin{aligned}
		y_j + x'_j &\leq \beta_j        &
		y_j &+ x'_j \geq 0 \\
		x'_j       &\leq 0       & 
		x'_j       &\geq \alpha_j \\
		\hat{y}_j  &\leq \gamma_j       &
		\hat{y}_j  &\geq 0 \\
		\hat{y}_j  &\leq y_j + x'_j &
		\hat{y}_j  &\geq y_j + x'_j  \\
		\hat{y}_j  &\leq -x'_j + \beta_j &
		\hat{y}_j  &\geq -x'_j + \alpha_j \\
		\hat{y}_j  &\leq y_j  &
		\hat{y}_j  &\geq y_j - \gamma_j
	\end{aligned}
\end{align*} Now we can see, $y_j+x'_j\geq 0$ and $x'_j \leq 0$ (lines 1\&2), hence $y_j \geq 0$; and $\hat{y}_j= y_j + x'_j$ (line 4). 

By above discussing,  we have: \begin{align*}
	& \begin{aligned}
		\hat{y}_j  \leq& y_j+x'_j \leq y_j  &\hat{y}_j  \geq& y_j+x'_j \geq 0
	\end{aligned}
\end{align*}

Then by the assumption of the proposition that $y_j \in [-\gamma_j, \gamma_j]$ and $x'_j,y_j+x'_j \in [\alpha_j,\beta_j]$, all 3 other lines are implied by the following inequalities respectively (one for one): \begin{align*}
	& \begin{aligned}
		\hat{y}_j  \leq&  y_j \leq \gamma_j       &
		\hat{y}_j  \geq& y_j+x'_j \geq 0 \\
		\hat{y}_j  \leq& 0 \leq -x'_j + \beta_j &
		\hat{y}_j  \geq& 0 \geq -x'_j + \alpha_j \\
		\hat{y}_j  \leq& y_j+x'_j \leq y_j  &
		\hat{y}_j  \geq& 0 \geq y_j - \gamma_j
	\end{aligned}
\end{align*}Therefore all 3 rest lines are tautology.
	

	
\textbf{$\mathbf{a = 0, a' = 1}$:}  In this case, the inequalities become: \begin{align*}
	& \begin{aligned}
		y_j + x'_j &\leq 0        &
		y_j &+ x'_j \geq \alpha_j \\
		x'_j       &\leq \beta_j       & 
		x'_j       &\geq 0 \\
		\hat{y}_j  &\leq 0      &
		\hat{y}_j  &\geq -\gamma_j \\
		\hat{y}_j  &\leq y_j + x'_j - \alpha_j &
		\hat{y}_j  &\geq y_j + x'_j  -\beta_j\\
		\hat{y}_j  &\leq -x'_j &
		\hat{y}_j  &\geq -x'_j \\
		\hat{y}_j  &\leq y_j + \gamma_j  &
		\hat{y}_j  &\geq y_j
	\end{aligned}
\end{align*} Now we can see, $y_j+x'_j\leq 0$ and $x'_j \geq 0$ (lines 1\&2), hence $y_j \leq 0$; and $\hat{y}_j= - x'_j$ (line 5). 

By above discussing,  we have: \begin{align*}
	& \begin{aligned}
		\hat{y}_j  &\leq -x'_j\leq 0      & \hspace*{4ex}
		\hat{y}_j  &\geq -x'_j \geq -x'_j+(y_j+x'_j) \geq y_j
	\end{aligned}
\end{align*}

Then by the assumption of the proposition that $y_j \in [-\gamma_j, \gamma_j]$ and $x'_j,y_j+x'_j \in [\alpha_j,\beta_j]$, all 3 other lines are implied by the following inequalities respectively (one for one):\begin{align*}
	& \begin{aligned}
		\hat{y}_j  &\leq -x'_j\leq 0      &
		\hat{y}_j  &\geq y_j\geq -\gamma_j \\
		\hat{y}_j  &\leq 0 \leq y_j + x'_j - \alpha_j &
		\hat{y}_j  &\geq y_j \geq y_j + x'_j -\beta_j \\
		\hat{y}_j  &\leq 0 \leq y_j + \gamma_j  &
		\hat{y}_j  &\geq  y_j
	\end{aligned}
\end{align*}Therefore all 3 rest lines are tautology.




	
\textbf{$\mathbf{a = 1, a' = 1}$:} In this case, the inequalities become: \begin{align*}
	& \begin{aligned}
		y_j + x'_j &\leq \beta_j        &
		y_j &+ x'_j \geq 0 \\
		x'_j       &\leq \beta_j       & 
		x'_j       &\geq 0 \\
		\hat{y}_j  &\leq \gamma_j       &
		\hat{y}_j  &\geq -\gamma_j \\
		\hat{y}_j  &\leq y_j + x'_j  &
		\hat{y}_j  &\geq y_j + x'_j - \beta_j \\
		\hat{y}_j  &\leq -x'_j + \beta_j &
		\hat{y}_j  &\geq -x'_j \\
		\hat{y}_j  &\leq y_j &
		\hat{y}_j  &\geq y_j
	\end{aligned}
\end{align*} Now we can see, $y_j+x'_j\geq 0$ and $x'_j \geq 0$ (lines 1\&2) and $\hat{y}_j= y_j$ (line 6). 


Then by the assumption of the proposition that $y_j \in [-\gamma_j, \gamma_j]$ and $x'_j,y_j+x'_j \in [\alpha_j,\beta_j]$, all 3 other lines are implied by the following inequalities respectively (one for one):\begin{align*}
	& \begin{aligned}
		\hat{y}_j  &\leq y_j\leq \gamma_j       &
		\hat{y}_j  &\geq y_j\geq -\gamma_j \\
		\hat{y}_j  &\leq y_j \leq y_j + x'_j  &
		\hat{y}_j  &\geq y_j \geq y_j + x'_j - \beta_j \\
		\hat{y}_j  &\leq -x'_j+(y_j+x'_j)\leq -x'_j + \beta_j &
		\hat{y}_j  &\geq y_j - (y_j+x'_j)\geq -x'_j \\
	\end{aligned}
\end{align*}Therefore all 3 rest lines are tautology.
	
	\qed
\end{proof}



\begin{proof}[of Proposition 3] First, we list the inequalities: \begin{align*}
		\hat{y}_i &\leq a \gamma_i               &\quad \hat{y}_i &\geq y_i - a \gamma_i \\
		\hat{y}_i &\geq (a-1) \gamma_i           &\quad \hat{y}_i &\leq y_i + (1-a) \gamma_i
	\end{align*}
	
	Similar to Proposition 2, we consider by cases.
	
	\textbf{$\mathbf{a = 0}$:} In this case, the inequalities become: \begin{align*}
		\hat{y}_i &\leq 0               &\quad \hat{y}_i &\geq y_i \\
		\hat{y}_i &\geq -\gamma_i           &\quad \hat{y}_i &\leq y_i + \gamma_i
	\end{align*} Now we can see, $y_i\leq 0$ (line 1). Line 2 becomes tautology since \begin{align*}
	\hat{y}_i &\geq y_i \geq -\gamma_i           &\quad \hat{y}_i &\leq 0 \leq y_i + \gamma_i
	\end{align*}

	\textbf{$\mathbf{a = 1}$:} In this case, the inequalities become: \begin{align*}
		\hat{y}_i &\leq \gamma_i               &\quad \hat{y}_i &\geq y_i - \gamma_i \\
		\hat{y}_i &\geq 0           &\quad \hat{y}_i &\leq y_i 
	\end{align*} Now we can see, $y_i\geq 0$ (line 2). Line 1 becomes tautology since \begin{align*}
	\hat{y}_i &\leq y_i\leq \gamma_i               &\quad \hat{y}_i &\geq 0 \geq y_i - \gamma_i 
	\end{align*}
		
Now we finish the proof. \qed
\end{proof}